shitpost

LeanPlayground/UnivAlg/Basics.lean
@@ -7,6 +7,112 @@
 
 
 
+/- SECTION: Utilities -/
+
+/-- `Vec n α : Type u` is the `n : Nat`-fold iterated product of `α : Type u`. -/
+def Vec.{u} : Nat → Type u → Type u
+  | 0,       _ => PUnit
+  | .succ n, α => α × Vec n α
+
+def makeVecFunctor : (n : Nat) → Functor (Vec n)
+  | 0 => { map := fun _ _ => () }
+  | .succ n => { map := fun f (a, as) => (f a, (makeVecFunctor n).map f as) }
+instance instVecFunctor {n : Nat} : Functor (Vec n) where map := (makeVecFunctor n).map
+
+def List.toVec.{u} {α : Type u} : (xs : List α) → Vec xs.length α
+  | [] => PUnit.unit
+  | (x :: xs) => (x, xs.toVec)
+
+/--
+  Given `xs : List α` and a function `f : {x : α // x ∈ xs} → β` acting on the members of `xs`,
+  map `f` over `xs` to produce a `List β`.
+
+  `smap` is short for `s`ubtype `map`.
+-/
+def List.smap.{u, u'} {α : Type u} {β : Type u'} (xs : List α) (f : {x : α // x ∈ xs} → β) : List β :=
+  match xs with
+  | [] => []
+  | (x :: xs') =>
+    have : x ∈ x :: xs' := List.mem_cons_self ..
+    f ⟨x, ‹_›⟩ :: xs'.smap (fun ⟨y, h⟩ => f ⟨y, List.mem_cons.mpr (.inr h)⟩)
+
+theorem List.smap_nil.{u, u'}
+  {α : Type u} {β : Type u'}
+  (f : {x : α // x ∈ []} → β)
+  : [].smap f = []
+  := rfl
+theorem List.smap_cons.{u, u'}
+  {α : Type u} {β : Type u'}
+  (x : α) (xs : List α)
+  (f : {a : α // a ∈ (x :: xs)} → β)
+  : (x :: xs).smap f = f ⟨x, List.mem_cons_self ..⟩ :: xs.smap (fun ⟨y, h⟩ => f ⟨y, List.mem_cons.mpr (.inr h)⟩)
+  := rfl
+
+theorem List.length_smap.{u, u'}
+  {α : Type u} {β : Type u'}
+  (xs : List α)
+  (f : {x : α // x ∈ xs} → β)
+  : (xs.smap f).length = xs.length
+  := by
+    induction xs
+    case nil => rfl
+    case cons x xs ih => rw [List.length_cons, List.smap_cons, List.length_cons, ih]
+
+theorem List.mem_smap.{u, u'}
+  {α : Type u} {β : Type u'}
+  {xs : List α}
+  {f : {x : α // x ∈ xs} → β}
+  {b : β}
+  : b ∈ xs.smap f
+  ↔ ∃ (a : { x // x ∈ xs }), f a = b
+  := by
+    constructor
+    case mp =>
+      induction xs
+      case nil =>
+        intro h
+        contradiction -- `b ∈ [].smap f` is `b ∈ []` is `False`
+      case cons x xs ih =>
+        intro h
+        rw [List.smap_cons, List.mem_cons] at h
+        cases h
+        case inl h =>
+          have : x ∈ x :: xs := List.mem_cons.mpr (.inl rfl)
+          exists ⟨x, ‹_›⟩
+          rw [h]
+        case inr h =>
+          have ⟨⟨a, _⟩, _⟩ := ih h
+          have : a ∈ x :: xs := mem_cons.mpr (.inr ‹a ∈ xs›)
+          exists ⟨a, ‹_›⟩
+    case mpr =>
+      intro ⟨⟨x, h_x⟩, h_fx⟩
+      induction xs
+      case nil =>
+        contradiction -- `h_x : x ∈ []`
+      case cons y ys ih =>
+        have := h_x
+        rw [mem_cons] at this
+        rw [smap_cons, mem_cons]
+        cases this
+        case inl h_x' => -- `h_x' : x = y`
+          apply Or.inl
+          rw [←h_fx]
+          have : (⟨x, h_x⟩ : {a // a ∈ y :: ys}) = ⟨y, mem_cons_self y ys⟩ := by
+            apply Subtype.eq
+            show x = y
+            exact ‹x = y›
+          rw [this]
+        case inr h_x =>
+          apply Or.inr
+          let f' : { x // x ∈ ys } → β := (fun x => f ⟨x.val, mem_cons.mpr (Or.inr x.property)⟩)
+          show b ∈ ys.smap f'
+          have := @ih f' h_x
+          apply this
+          rw [←h_fx]
+
+
+
+
 /- SECTION: Equational classes (but not their models) -- inital definitions and setup -/
 
 /-- A logical operation (function symbol), specified by an `.id` and `.arity`. -/
@@ -14,15 +120,152 @@ structure Operation : Type where
   id    : String
   arity : Nat
 deriving Repr
+@[inherit_doc Operation]
 abbrev Op : Type := Operation
 
-/-- A list of operations, each with unique `.id`s. -/
-structure Operations : Type where
-  list : List Operation
-  uqIds : ∀ (i j : Fin list.length), i ≠ j → list.get i ≠ list.get j
+/-- A list of elements which return distinct values according to a discriminating function. -/
+structure UniqueList.{u, u'} (α : Type u) {β : Type u'} (discriminate : α → β) : Type u where
+  list : List α
+  uq : ∀ (i j : Fin list.length), i ≠ j → discriminate (list.get i) ≠ discriminate (list.get j)
 deriving Repr
-abbrev Ops : Type := Operations
+@[inherit_doc UniqueList]
+abbrev UqList := UniqueList
+instance instMemUqList : Membership α (UqList α d) where
+  mem uαs a := a ∈ uαs.list
 
--- TODO:
---  Equations between operation composites in an operation list
---  Equational classes
+/-- A list of operations, each with unique `.id`s. -/
+def Operations : Type := UniqueList Operation Operation.id
+deriving Repr
+/-- The underlying list of operations. -/
+def Operations.list : Operations → List Operation := UniqueList.list
+/-- A proof that the operation IDs are distinct. -/
+def Operations.uqIds
+  : (ops : Operations)
+  → (∀ (i j : Fin ops.list.length), i ≠ j → (ops.list.get i).id ≠ (ops.list.get j).id)
+  := UniqueList.uq
+@[inherit_doc Operations]
+abbrev Ops : Type := Operations
+instance instCoeOpsListOp : Coe Ops (List Op) where
+  coe ops := ops.list
+instance instMemOpOps : Membership Op Ops where
+  mem ops op := op ∈ ops.list
+
+/-- A list of distinct variable names. -/
+def Variables : Type := UniqueList String id
+deriving Repr
+/-- The underlying list of variable names. -/
+def Variables.list : Variables → List String := UniqueList.list
+/-- A proof that the variable names are unique. -/
+def Variables.uq
+  : (vars : Variables)
+  → (∀ (i j : Fin vars.list.length), i ≠ j → vars.list.get i ≠ vars.list.get j) := UniqueList.uq
+@[inherit_doc Variables]
+abbrev Vars : Type := Variables
+instance instCoeVarsListString : Coe Vars (List String) where
+  coe := Variables.list
+instance instMemStringVars : Membership String Vars where
+  mem vars string := string ∈ vars.list
+
+-- FIXME: I'm pretty sure that I just need to completely rethink the structure of `Term`s here.
+--  It's currently really messy, and hard to reason with in Lean4 (no `Term.brecOn`, so termination proofs
+--  are awful).
+-- It's a real shame that I can't have `Vec op.arity Term` as part of the `inductive` definition :/
+/--
+  The structure behind a term, but with no guarantee that it makes any sense.
+  A term is comprised of `Var`iables with given `String` names, and `App`lications
+  of `Operation` symbols to other terms.
+
+  In `App op args`, `op` might not appear in `ops` and `args.length`
+  might not be equal to `op.arity`.
+  See also `Term`, which consists of only *legal* terms.
+  See also `Term'.isLegal`.
+-/
+inductive Term' (ops : Ops) (vars : Vars) : Type where
+  | var : (name : String) → Term' ops vars
+  | app : (op : Op) → (args : List (Term' ops vars)) → Term' ops vars
+deriving Repr
+/-- Specification for whether a given `Term' ops` is legal. -/
+def Term'.isLegal (ops : Ops) (vars : Vars) : Term' ops vars → Prop
+  | var v       => v ∈ vars
+  | app op args => (op ∈ ops) ∧ (args.length = op.arity) ∧ (∀ (a : Term' ops vars), a ∈ args → a.isLegal)
+/-- A legal term over a given language `ops : Ops` of operations with variable names found in `vars : Vars`. -/
+def Term (ops : Ops) (vars : Vars) : Type := { t : Term' ops vars // t.isLegal }
+
+/-- An equation, consisting of a `Term` on the `lhs` of the equation, and another on its `rhs`. -/
+structure Equation (ops : Ops) (vars : Vars) : Type where
+  lhs : Term ops vars
+  rhs : Term ops vars
+
+/--
+  An **equational class** -- a system with a language of function symbols and axioms
+  encoded as universally quantified equations among legal composites of these function
+  symbols.
+
+  `ops  : Ops`  describes the list of operations in the class.
+  `vars : Vars` describes the list of variable names universally quantified over in the list of equations.
+  `eqs  : List (Equation ops vars)` is the list of equations to be satisfied in the equational class.
+-/
+structure EquationalClass : Type where
+  ops  : Ops
+  vars : Vars
+  eqs  : List (Equation ops vars)
+
+
+
+/- SECTION: Models of equational classes -/
+
+/--
+  Given a `carrier` type and some interpretations `opsInt` of specified `ops : Ops` as genuine operations
+  on the `carrier`, interpret a `Term` as a function mapping a choice for the free variables in the `Term`
+  to an element of the `carrier`.
+-/
+noncomputable -- code generator doesn't support `Subtype.recOn` yet :/
+def Term.interpret.{u}
+  {ops : Ops}
+  {vars : Vars}
+  (carrier : Type u)
+  (opsInt : (op : { o : Op // o ∈ ops }) → (Vec op.val.arity carrier) → carrier)
+  (term : Term ops vars)
+  (subs : { v : String // v ∈ vars } → carrier)
+  : carrier
+  := term.recOn <| fun val =>
+    match val with
+    | .var v => fun p =>
+      have : v ∈ vars := by {
+        unfold Term'.isLegal at p
+        exact p
+      }
+      subs ⟨v, ‹_›⟩
+    | .app op args => fun p =>
+      have : op ∈ ops := by {
+        unfold Term'.isLegal at p
+        exact p.left
+      }
+      have h_args_legal : ∀ (a : Term' ops vars), a ∈ args → a.isLegal ops vars := by {
+        unfold Term'.isLegal at p
+        exact p.right.right
+      }
+      let arg2Term : {a : Term' ops vars // a ∈ args} → Term ops vars :=
+        fun a =>
+        have : a.val.isLegal ops vars := h_args_legal a.val a.property
+        ⟨a, ‹_›⟩
+      let legalArgs : List (Term ops vars) := List.smap args arg2Term
+      -- FIXME: This is the recursive call that's eating my ass
+      let argVals : List carrier := legalArgs.smap (Term.interpret carrier opsInt · subs)
+      have : argVals.length = op.arity := by {
+        unfold argVals
+        rw [List.length_smap]
+        unfold legalArgs
+        rw [List.length_smap]
+        unfold Term'.isLegal at p
+        exact p.right.left
+      }
+      let vecVals : Vec op.arity carrier := (this ▸ argVals.toVec)
+      opsInt ⟨op, ‹_›⟩ vecVals
+  termination_by term.val
+  decreasing_by (repeat sorry)
+
+-- structure Model.{u} (eqc : EquationalClass) where
+--   carrier : Type u
+--   ops : (op : { o : Op // o ∈ eqc.ops }) → (Vec op.val.arity carrier) → carrier
+--   eqs : (eq : { e : Equation eqc.ops eqc.vars // e ∈ eqc.eqs }) → sorry -- FIXME: Codify a statement of the equation
